@prefix : <https://knb.ecoinformatics.org/knb/streamnet/rpers/lod/ontology/> .
@prefix owl: <http://www.w3.org/2002/07/owl#> .
@prefix rdf: <http://www.w3.org/1999/02/22-rdf-syntax-ns#> .
@prefix xml: <http://www.w3.org/XML/1998/namespace> .
@prefix xsd: <http://www.w3.org/2001/XMLSchema#> .
@prefix rdfs: <http://www.w3.org/2000/01/rdf-schema#> .
@prefix sosa: <http://www.w3.org/ns/sosa/> .
@prefix fish-ont: <http://purl.dataone.org/odo/fish-ont/> .
@prefix oboe-core: <http://ecoinformatics.org/oboe/oboe.1.2/oboe-core.owl#> .
@prefix rpers-ont: <https://knb.ecoinformatics.org/knb/streamnet/rpers/lod/ontology/> .
@prefix streamnet-ont: <https://knb.ecoinformatics.org/knb/streamnet/lod/ontology/> .
@base <https://knb.ecoinformatics.org/knb/streamnet/rpers/lod/ontology/> .

<https://knb.ecoinformatics.org/knb/streamnet/rpers/lod/ontology/> rdf:type owl:Ontology .

#################################################################
#    Object Properties
#################################################################

###  http://purl.dataone.org/odo/fish-ont/associatedPopulation
fish-ont:associatedPopulation rdf:type owl:ObjectProperty ;
                              rdfs:label "associated population" .


###  http://purl.dataone.org/odo/fish-ont/associatedRegion
fish-ont:associatedRegion rdf:type owl:ObjectProperty ;
                          rdfs:label "associated region" .


###  http://purl.dataone.org/odo/fish-ont/broodingYear
fish-ont:broodingYear rdf:type owl:ObjectProperty ;
                      rdfs:subPropertyOf fish-ont:hasTemporalContext ;
                      rdfs:label "brooding year" .


###  http://purl.dataone.org/odo/fish-ont/hasTemporalContext
fish-ont:hasTemporalContext rdf:type owl:ObjectProperty ;
                            rdfs:label "has temporal context" .


###  http://purl.dataone.org/odo/fish-ont/locatedIn
fish-ont:locatedIn rdf:type owl:ObjectProperty ;
                   rdfs:label "located in" .


###  http://purl.dataone.org/odo/fish-ont/ofSpeciesType
fish-ont:ofSpeciesType rdf:type owl:ObjectProperty ;
                       rdfs:label "of species type" .


###  https://knb.ecoinformatics.org/knb/streamnet/lod/ontology/fallsUnderRegion
streamnet-ont:fallsUnderRegion rdf:type owl:ObjectProperty ;
                               rdfs:label "falls under region" .


#################################################################
#    Data properties
#################################################################

###  https://knb.ecoinformatics.org/knb/streamnet/lod/ontology/commonPopulationName
streamnet-ont:commonPopulationName rdf:type owl:DatatypeProperty ;
                                   rdfs:comment "Population name used by local biologists." ;
                                   rdfs:label "common population name" .


###  https://knb.ecoinformatics.org/knb/streamnet/lod/ontology/escapementName
streamnet-ont:escapementName rdf:type owl:DatatypeProperty ;
                             rdfs:label "escapement name" .


###  https://knb.ecoinformatics.org/knb/streamnet/lod/ontology/escapementTiming
streamnet-ont:escapementTiming rdf:type owl:DatatypeProperty ;
                               rdfs:comment "Specific time period (months) for an escapement estimate." ;
                               rdfs:label "escapement timing" .


###  https://knb.ecoinformatics.org/knb/streamnet/lod/ontology/esu_dps
streamnet-ont:esu_dps rdf:type owl:DatatypeProperty ;
                      rdfs:comment "For ESA-listed populations , the Evolutionarily Significant Unit / Distinct Population Segment defined by NMFS / USFWS.  For non-listed populations this is the DPS or other name." ;
                      rdfs:label "esu dps" .


###  https://knb.ecoinformatics.org/knb/streamnet/lod/ontology/locationName
streamnet-ont:locationName rdf:type owl:DatatypeProperty ;
                           rdfs:comment "Location part of ESApopName." ;
                           rdfs:label "location name" .


###  https://knb.ecoinformatics.org/knb/streamnet/lod/ontology/methodID
streamnet-ont:methodID rdf:type owl:DatatypeProperty ;
                       rdfs:comment "When an organization provides > 1 estimate per year, this number identifies which method was used." ;
                       rdfs:label "method number" .


###  https://knb.ecoinformatics.org/knb/streamnet/lod/ontology/methodName
streamnet-ont:methodName rdf:type owl:DatatypeProperty ;
                         rdfs:comment "Name(s) of protocols, data collection, and data analysis methods used to calculate the indicator estimate." ;
                         rdfs:label "protocol method name" .


###  https://knb.ecoinformatics.org/knb/streamnet/lod/ontology/methodSource_URL
streamnet-ont:methodSource_URL rdf:type owl:DatatypeProperty ;
                               rdfs:comment "Links to protocols and methods describing the methodology and documenting the derivation of the indicator." ;
                               rdfs:label "method URL" .


###  https://knb.ecoinformatics.org/knb/streamnet/lod/ontology/nmfs_majorPopulationGroup
streamnet-ont:nmfs_majorPopulationGroup rdf:type owl:DatatypeProperty ;
                                        rdfs:comment "\"Major population group\" or “stratum” (defined by NMFS), in which the population falls." ;
                                        rdfs:label "nmfs population group" .


###  https://knb.ecoinformatics.org/knb/streamnet/lod/ontology/nmfs_populationID
streamnet-ont:nmfs_populationID rdf:type owl:DatatypeProperty ;
                                rdfs:comment "NMFS code for the population of fish." ;
                                rdfs:label "nmfs population code" .


###  https://knb.ecoinformatics.org/knb/streamnet/lod/ontology/nmfs_populationName
streamnet-ont:nmfs_populationName rdf:type owl:DatatypeProperty ;
                                  rdfs:comment "Population name used by NMFS." ;
                                  rdfs:label "nmfs population name" .


###  https://knb.ecoinformatics.org/knb/streamnet/lod/ontology/populationFitNotes
streamnet-ont:populationFitNotes rdf:type owl:DatatypeProperty ;
                                 rdfs:comment "Text description of why the data are not at the scale of a single population." ;
                                 rdfs:label "population fit notes" .


###  https://knb.ecoinformatics.org/knb/streamnet/lod/ontology/streamnet_populationID
streamnet-ont:streamnet_populationID rdf:type owl:DatatypeProperty ;
                                     rdfs:comment "StreamNet code for the population of fish." ;
                                     rdfs:label "streamnet population ID" .


###  https://knb.ecoinformatics.org/knb/streamnet/lod/ontology/streamnet_populationName
streamnet-ont:streamnet_populationName rdf:type owl:DatatypeProperty ;
                                       rdfs:comment "Population name used by StreamNet." ;
                                       rdfs:label "streamnet population name" .


###  https://knb.ecoinformatics.org/knb/streamnet/rpers/lod/ontology/rpersDefinition
rpers-ont:rpersDefinition rdf:type owl:DatatypeProperty ;
                          rdfs:label "rpers definition" .


###  https://knb.ecoinformatics.org/knb/streamnet/rpers/lod/ontology/rpersType
rpers-ont:rpersType rdf:type owl:DatatypeProperty ;
                    rdfs:label "rpers type" .


#################################################################
#    Classes
#################################################################

###  http://ecoinformatics.org/oboe/oboe.1.2/oboe-core.owl#Characteristic
oboe-core:Characteristic rdf:type owl:Class .


###  http://ecoinformatics.org/oboe/oboe.1.2/oboe-core.owl#Entity
oboe-core:Entity rdf:type owl:Class .


###  http://ecoinformatics.org/oboe/oboe.1.2/oboe-core.owl#Measurement
oboe-core:Measurement rdf:type owl:Class .


###  http://ecoinformatics.org/oboe/oboe.1.2/oboe-core.owl#Observation
oboe-core:Observation rdf:type owl:Class .


###  http://ecoinformatics.org/oboe/oboe.1.2/oboe-core.owl#ObservationCollection
oboe-core:ObservationCollection rdf:type owl:Class .


###  http://ecoinformatics.org/oboe/oboe.1.2/oboe-core.owl#Protocol
oboe-core:Protocol rdf:type owl:Class .


###  http://purl.dataone.org/odo/fish-ont/FishPopulation
fish-ont:FishPopulation rdf:type owl:Class .


###  http://www.opengis.net/ont/geosparql#Feature
<http://www.opengis.net/ont/geosparql#Feature> rdf:type owl:Class .


###  http://www.w3.org/ns/sosa/FeatureOfInterest
sosa:FeatureOfInterest rdf:type owl:Class .


###  http://www.w3.org/ns/sosa/ObservableProperty
sosa:ObservableProperty rdf:type owl:Class .


###  http://www.w3.org/ns/sosa/Observation
sosa:Observation rdf:type owl:Class .


###  http://www.w3.org/ns/sosa/ObservationCollection
sosa:ObservationCollection rdf:type owl:Class .


###  http://www.w3.org/ns/sosa/Procedure
sosa:Procedure rdf:type owl:Class .


###  https://knb.ecoinformatics.org/knb/streamnet/lod/ontology/EstimationProtocol
streamnet-ont:EstimationProtocol rdf:type owl:Class ;
                                 rdfs:subClassOf oboe-core:Protocol ,
                                                 sosa:Procedure ;
                                 rdfs:label "Estimation Protocol (Streamnet)" .


###  https://knb.ecoinformatics.org/knb/streamnet/lod/ontology/RecoveryDomain
streamnet-ont:RecoveryDomain rdf:type owl:Class ;
                             rdfs:subClassOf <http://www.opengis.net/ont/geosparql#Feature> ;
                             rdfs:label "Recovery Domain" .


###  https://knb.ecoinformatics.org/knb/streamnet/lod/ontology/RecruitLocation
streamnet-ont:RecruitLocation rdf:type owl:Class ;
                              rdfs:subClassOf oboe-core:Entity ,
                                              <http://www.opengis.net/ont/geosparql#Feature> ,
                                              sosa:FeatureOfInterest ;
                              rdfs:comment "Specific named location(s) where the recruit abundance numbers were determined." ;
                              rdfs:label "Recruit Location (Streamnet)" .


###  https://knb.ecoinformatics.org/knb/streamnet/lod/ontology/RunType
streamnet-ont:RunType rdf:type owl:Class ;
                      rdfs:label "Run Type (Streamnet)" .


###  https://knb.ecoinformatics.org/knb/streamnet/lod/ontology/SalmonMeasurementCharacteristic
streamnet-ont:SalmonMeasurementCharacteristic rdf:type owl:Class ;
                                              rdfs:subClassOf oboe-core:Characteristic ,
                                                              sosa:ObservableProperty ;
                                              rdfs:label "Salmon Measurement Characteristic (Streamnet)" .


###  https://knb.ecoinformatics.org/knb/streamnet/lod/ontology/SpawnerLocation
streamnet-ont:SpawnerLocation rdf:type owl:Class ;
                              rdfs:subClassOf oboe-core:Entity ,
                                              <http://www.opengis.net/ont/geosparql#Feature> ,
                                              sosa:FeatureOfInterest ;
                              rdfs:comment "Specific named location(s) where the spawner abundance numbers were determined." ;
                              rdfs:label "Spawner Location (Streamnet)" .


###  https://knb.ecoinformatics.org/knb/streamnet/rpers/lod/ontology/Escapement_Measurement
rpers-ont:Escapement_Measurement rdf:type owl:Class ;
                                 rdfs:subClassOf oboe-core:Measurement ;
                                 rdfs:label "Escapement Measurement (RperS)" .


###  https://knb.ecoinformatics.org/knb/streamnet/rpers/lod/ontology/Escapement_Observation
rpers-ont:Escapement_Observation rdf:type owl:Class ;
                                 rdfs:subClassOf oboe-core:Observation ,
                                                 sosa:Observation ;
                                 rdfs:label "Escapement Observation (RperS)" .


###  https://knb.ecoinformatics.org/knb/streamnet/rpers/lod/ontology/Escapement_ObservationCollection
rpers-ont:Escapement_ObservationCollection rdf:type owl:Class ;
                                           rdfs:subClassOf oboe-core:ObservationCollection ,
                                                           sosa:ObservationCollection ;
                                           rdfs:label "Escapement Observation Collection (RperS)" .


###  https://knb.ecoinformatics.org/knb/streamnet/rpers/lod/ontology/SalmonMeasurementCharacteristic
rpers-ont:SalmonMeasurementCharacteristic rdf:type owl:Class ;
                                          rdfs:subClassOf streamnet-ont:SalmonMeasurementCharacteristic ;
                                          rdfs:label "Salmon Measurement Characteristic (RperS)" .


###  https://knb.ecoinformatics.org/knb/streamnet/rpers/lod/ontology/SalmonPopulation
rpers-ont:SalmonPopulation rdf:type owl:Class ;
                           rdfs:subClassOf fish-ont:FishPopulation ;
                           rdfs:label "Salmon Population (RperS)" .


#################################################################
#    Individuals
#################################################################

###  https://knb.ecoinformatics.org/knb/streamnet/lod/ontology/runType.Early
streamnet-ont:runType.Early rdf:type owl:NamedIndividual ,
                                     streamnet-ont:RunType ;
                            rdfs:label "Early" .


###  https://knb.ecoinformatics.org/knb/streamnet/lod/ontology/runType.Early-Late
streamnet-ont:runType.Early-Late rdf:type owl:NamedIndividual ,
                                          streamnet-ont:RunType ;
                                 rdfs:label "Both early & late" .


###  https://knb.ecoinformatics.org/knb/streamnet/lod/ontology/runType.Fall
streamnet-ont:runType.Fall rdf:type owl:NamedIndividual ,
                                    streamnet-ont:RunType ;
                           rdfs:label "Fall" .


###  https://knb.ecoinformatics.org/knb/streamnet/lod/ontology/runType.Late
streamnet-ont:runType.Late rdf:type owl:NamedIndividual ,
                                    streamnet-ont:RunType ;
                           rdfs:label "Late" .


###  https://knb.ecoinformatics.org/knb/streamnet/lod/ontology/runType.LateFall
streamnet-ont:runType.LateFall rdf:type owl:NamedIndividual ,
                                        streamnet-ont:RunType ;
                               rdfs:label "Late Fall" .


###  https://knb.ecoinformatics.org/knb/streamnet/lod/ontology/runType.Spring
streamnet-ont:runType.Spring rdf:type owl:NamedIndividual ,
                                      streamnet-ont:RunType ;
                             rdfs:label "Spring" .


###  https://knb.ecoinformatics.org/knb/streamnet/lod/ontology/runType.Spring-Summer
streamnet-ont:runType.Spring-Summer rdf:type owl:NamedIndividual ,
                                             streamnet-ont:RunType ;
                                    rdfs:label "Spring summer" .


###  https://knb.ecoinformatics.org/knb/streamnet/lod/ontology/runType.Summer
streamnet-ont:runType.Summer rdf:type owl:NamedIndividual ,
                                      streamnet-ont:RunType ;
                             rdfs:label "Summer" .


###  https://knb.ecoinformatics.org/knb/streamnet/lod/ontology/runType.Summer-Winter
streamnet-ont:runType.Summer-Winter rdf:type owl:NamedIndividual ,
                                             streamnet-ont:RunType ;
                                    rdfs:label "Both summer & winter" .


###  https://knb.ecoinformatics.org/knb/streamnet/lod/ontology/runType.Unknown
streamnet-ont:runType.Unknown rdf:type owl:NamedIndividual ,
                                       streamnet-ont:RunType ;
                              rdfs:label "Unknown" .


###  https://knb.ecoinformatics.org/knb/streamnet/lod/ontology/runType.Winter
streamnet-ont:runType.Winter rdf:type owl:NamedIndividual ,
                                      streamnet-ont:RunType ;
                             rdfs:label "Winter" .


###  https://knb.ecoinformatics.org/knb/streamnet/rpers/lod/ontology/salmonCharacteristic.AGE10ADULTS
rpers-ont:salmonCharacteristic.AGE10ADULTS rdf:type owl:NamedIndividual ,
                                                    rpers-ont:SalmonMeasurementCharacteristic ;
                                           rdfs:comment "Total number of adult recruits that were age 10 (brood year +10)." ;
                                           rdfs:label "Age10Adults" .


###  https://knb.ecoinformatics.org/knb/streamnet/rpers/lod/ontology/salmonCharacteristic.AGE1JUVS
rpers-ont:salmonCharacteristic.AGE1JUVS rdf:type owl:NamedIndividual ,
                                                 rpers-ont:SalmonMeasurementCharacteristic ;
                                        rdfs:comment "Total number of juvenile recruits that were age 1 (brood year +1)." ;
                                        rdfs:label "Age1Juvs" .


###  https://knb.ecoinformatics.org/knb/streamnet/rpers/lod/ontology/salmonCharacteristic.AGE2ADULTS
rpers-ont:salmonCharacteristic.AGE2ADULTS rdf:type owl:NamedIndividual ,
                                                   rpers-ont:SalmonMeasurementCharacteristic ;
                                          rdfs:comment "Total number of adult recruits that were age 2 (brood year +2)." ;
                                          rdfs:label "Age2Adults" .


###  https://knb.ecoinformatics.org/knb/streamnet/rpers/lod/ontology/salmonCharacteristic.AGE2JUVS
rpers-ont:salmonCharacteristic.AGE2JUVS rdf:type owl:NamedIndividual ,
                                                 rpers-ont:SalmonMeasurementCharacteristic ;
                                        rdfs:comment "Total number of juvenile recruits at age 2 (brood year +2)." ;
                                        rdfs:label "Age2Juvs" .


###  https://knb.ecoinformatics.org/knb/streamnet/rpers/lod/ontology/salmonCharacteristic.AGE3ADULTS
rpers-ont:salmonCharacteristic.AGE3ADULTS rdf:type owl:NamedIndividual ,
                                                   rpers-ont:SalmonMeasurementCharacteristic ;
                                          rdfs:comment "Total number of adult recruits that were age 3 (brood year +3)." ;
                                          rdfs:label "Age3Adults" .


###  https://knb.ecoinformatics.org/knb/streamnet/rpers/lod/ontology/salmonCharacteristic.AGE3JUVS
rpers-ont:salmonCharacteristic.AGE3JUVS rdf:type owl:NamedIndividual ,
                                                 rpers-ont:SalmonMeasurementCharacteristic ;
                                        rdfs:comment "Total number of juvenile recruits at age 3 (brood year +3)." ;
                                        rdfs:label "Age3Juvs" .


###  https://knb.ecoinformatics.org/knb/streamnet/rpers/lod/ontology/salmonCharacteristic.AGE4ADULTS
rpers-ont:salmonCharacteristic.AGE4ADULTS rdf:type owl:NamedIndividual ,
                                                   rpers-ont:SalmonMeasurementCharacteristic ;
                                          rdfs:comment "Total number of adult recruits that were age 4 (brood year +4)." ;
                                          rdfs:label "Age4Adults" .


###  https://knb.ecoinformatics.org/knb/streamnet/rpers/lod/ontology/salmonCharacteristic.AGE4PLUSJUVS
rpers-ont:salmonCharacteristic.AGE4PLUSJUVS rdf:type owl:NamedIndividual ,
                                                     rpers-ont:SalmonMeasurementCharacteristic ;
                                            rdfs:comment "Total number of juvenile recruits at age 4 (brood year +4) or older." ;
                                            rdfs:label "Age4PlusJuvs" .


###  https://knb.ecoinformatics.org/knb/streamnet/rpers/lod/ontology/salmonCharacteristic.AGE5ADULTS
rpers-ont:salmonCharacteristic.AGE5ADULTS rdf:type owl:NamedIndividual ,
                                                   rpers-ont:SalmonMeasurementCharacteristic ;
                                          rdfs:comment "Total number of adult recruits that were age 5 (brood year +5)." ;
                                          rdfs:label "Age5Adults" .


###  https://knb.ecoinformatics.org/knb/streamnet/rpers/lod/ontology/salmonCharacteristic.AGE6ADULTS
rpers-ont:salmonCharacteristic.AGE6ADULTS rdf:type owl:NamedIndividual ,
                                                   rpers-ont:SalmonMeasurementCharacteristic ;
                                          rdfs:comment "Total number of adult recruits that were age 6 (brood year +6)." ;
                                          rdfs:label "Age6Adults" .


###  https://knb.ecoinformatics.org/knb/streamnet/rpers/lod/ontology/salmonCharacteristic.AGE7ADULTS
rpers-ont:salmonCharacteristic.AGE7ADULTS rdf:type owl:NamedIndividual ,
                                                   rpers-ont:SalmonMeasurementCharacteristic ;
                                          rdfs:comment "Total number of adult recruits that were age 7 (brood year +7)." ;
                                          rdfs:label "Age7Adults" .


###  https://knb.ecoinformatics.org/knb/streamnet/rpers/lod/ontology/salmonCharacteristic.AGE8ADULTS
rpers-ont:salmonCharacteristic.AGE8ADULTS rdf:type owl:NamedIndividual ,
                                                   rpers-ont:SalmonMeasurementCharacteristic ;
                                          rdfs:comment "Total number of adult recruits that were age 8 (brood year +8)." ;
                                          rdfs:label "Age8Adults" .


###  https://knb.ecoinformatics.org/knb/streamnet/rpers/lod/ontology/salmonCharacteristic.AGE9ADULTS
rpers-ont:salmonCharacteristic.AGE9ADULTS rdf:type owl:NamedIndividual ,
                                                   rpers-ont:SalmonMeasurementCharacteristic ;
                                          rdfs:comment "Total number of adult recruits that were age 9 (brood year +9)." ;
                                          rdfs:label "Age9Adults" .


###  https://knb.ecoinformatics.org/knb/streamnet/rpers/lod/ontology/salmonCharacteristic.HARVESTADJ
rpers-ont:salmonCharacteristic.HARVESTADJ rdf:type owl:NamedIndividual ,
                                                   rpers-ont:SalmonMeasurementCharacteristic ;
                                          rdfs:comment "How the return was adjusted to account for harvest. (Which harvested fish are included in the estimate of number of adults.)" ;
                                          rdfs:label "HarvestAdj" .


###  https://knb.ecoinformatics.org/knb/streamnet/rpers/lod/ontology/salmonCharacteristic.HATCHERYSPAWNERS
rpers-ont:salmonCharacteristic.HATCHERYSPAWNERS rdf:type owl:NamedIndividual ,
                                                         rpers-ont:SalmonMeasurementCharacteristic ;
                                                rdfs:comment "Number of parent spawners of hatchery origin that contributed to the brood year this record reflects." ;
                                                rdfs:label "HatcherySpawners" .


###  https://knb.ecoinformatics.org/knb/streamnet/rpers/lod/ontology/salmonCharacteristic.MAINSTEMHARVEST
rpers-ont:salmonCharacteristic.MAINSTEMHARVEST rdf:type owl:NamedIndividual ,
                                                        rpers-ont:SalmonMeasurementCharacteristic ;
                                               rdfs:comment "Number of adults and jacks from the recruit group indicated in the Recruits field that were harvested in the mainstem (including the estuary)." ;
                                               rdfs:label "MainstemHarvest" .


###  https://knb.ecoinformatics.org/knb/streamnet/rpers/lod/ontology/salmonCharacteristic.NOBROODSTOCKREMOVED
rpers-ont:salmonCharacteristic.NOBROODSTOCKREMOVED rdf:type owl:NamedIndividual ,
                                                            rpers-ont:SalmonMeasurementCharacteristic ;
                                                   rdfs:comment "Additional recruits that would have returned had there not been removal of fish from this brood year for use as broodstock in a hatchery." ;
                                                   rdfs:label "NOBroodStockRemoved" .


###  https://knb.ecoinformatics.org/knb/streamnet/rpers/lod/ontology/salmonCharacteristic.OCEANHARVEST
rpers-ont:salmonCharacteristic.OCEANHARVEST rdf:type owl:NamedIndividual ,
                                                     rpers-ont:SalmonMeasurementCharacteristic ;
                                            rdfs:comment "Number of adults and jacks from the recruit group indicated in the Recruits field that were harvested in the ocean." ;
                                            rdfs:label "OceanHarvest" .


###  https://knb.ecoinformatics.org/knb/streamnet/rpers/lod/ontology/salmonCharacteristic.RECRUITS
rpers-ont:salmonCharacteristic.RECRUITS rdf:type owl:NamedIndividual ,
                                                 rpers-ont:SalmonMeasurementCharacteristic ;
                                        rdfs:comment "Number of natural origin recruits from the indicated combination of species, run, population, spawner location, recruit location, brood year, and RperStype." ;
                                        rdfs:label "Recruits" .


###  https://knb.ecoinformatics.org/knb/streamnet/rpers/lod/ontology/salmonCharacteristic.RECRUITSMISSING
rpers-ont:salmonCharacteristic.RECRUITSMISSING rdf:type owl:NamedIndividual ,
                                                        rpers-ont:SalmonMeasurementCharacteristic ;
                                               rdfs:comment "Whether any recruits for this brood year were missing." ;
                                               rdfs:label "RecruitsMissing" .


###  https://knb.ecoinformatics.org/knb/streamnet/rpers/lod/ontology/salmonCharacteristic.RPERS
rpers-ont:salmonCharacteristic.RPERS rdf:type owl:NamedIndividual ,
                                              rpers-ont:SalmonMeasurementCharacteristic ;
                                     rdfs:comment "Ratio of recruits from the designated brood year and RperStype, divided by the number of parent spawners responsible for that brood year." ;
                                     rdfs:label "RperS" .


###  https://knb.ecoinformatics.org/knb/streamnet/rpers/lod/ontology/salmonCharacteristic.TOTALSPAWNERS
rpers-ont:salmonCharacteristic.TOTALSPAWNERS rdf:type owl:NamedIndividual ,
                                                      rpers-ont:SalmonMeasurementCharacteristic ;
                                             rdfs:comment "Total number of parent spawners, both natural and hatchery origin, that produced the brood year this record reflects." ;
                                             rdfs:label "TotalSpawners" .


###  https://knb.ecoinformatics.org/knb/streamnet/rpers/lod/ontology/salmonCharacteristic.TRIBHARVEST
rpers-ont:salmonCharacteristic.TRIBHARVEST rdf:type owl:NamedIndividual ,
                                                    rpers-ont:SalmonMeasurementCharacteristic ;
                                           rdfs:comment "Number of adults and jacks from the recruit group indicated in the Recruits field that were harvested in tributaries." ;
                                           rdfs:label "TribHarvest" .


###  https://knb.ecoinformatics.org/knb/streamnet/rpers/lod/ontology/salmonCharacteristic.YOY
rpers-ont:salmonCharacteristic.YOY rdf:type owl:NamedIndividual ,
                                            rpers-ont:SalmonMeasurementCharacteristic ;
                                   rdfs:comment "Total number of juvenile recruits (parr or smolts) at age 0 (brood year +0)." ;
                                   rdfs:label "YOY" .


###  Generated by the OWL API (version 4.5.29.2024-05-13T12:11:03Z) https://github.com/owlcs/owlapi
